Now with transition labes and inputs enumerated from 1.
Also, data registers are always initialised to Nil and have to be assigned to. However, arithmetic operators now treat Nil as 0, so you can do r1 := r1 + i1, for example.

formal/EFSM.thy
@@ -2,32 +2,32 @@ theory EFSM
 imports IO
 begin
 
-abbreviation is_possible_step :: "efsm \<Rightarrow> statename \<Rightarrow> statename \<Rightarrow> transition \<Rightarrow> inputs \<Rightarrow> data \<Rightarrow> bool" where
-"is_possible_step e s s' t ip dt \<equiv> 
-  ((find (\<lambda>x . x = t) (M e(s,s')) \<noteq> None) \<and> (fst t)(ip,dt))"
+abbreviation is_possible_step :: "efsm \<Rightarrow> statename \<Rightarrow> statename \<Rightarrow> transition \<Rightarrow> label \<Rightarrow> inputs \<Rightarrow> data \<Rightarrow> bool" where
+"is_possible_step e s s' t l ip dt \<equiv> 
+  (((label t) = l) \<and> (find (\<lambda>x . x = t) (M e(s,s')) \<noteq> None) \<and> (guard t)(ip,dt))"
 
-abbreviation possible_steps :: "efsm \<Rightarrow> statename \<Rightarrow> inputs \<Rightarrow> data \<Rightarrow> (statename * transition) list" where
-"possible_steps e s ip dt \<equiv> [(s',t) . s' \<leftarrow> S e, t \<leftarrow> M e(s,s'), is_possible_step e s s' t ip dt]"
+abbreviation possible_steps :: "efsm \<Rightarrow> statename \<Rightarrow> label \<Rightarrow> inputs \<Rightarrow> data \<Rightarrow> (statename * transition) list" where
+"possible_steps e s l ip dt \<equiv> [(s',t) . s' \<leftarrow> S e, t \<leftarrow> M e(s,s'), is_possible_step e s s' t l ip dt]"
 
-definition step :: "efsm \<Rightarrow> statename \<Rightarrow> inputs \<Rightarrow> data \<Rightarrow> (statename \<times> outvalues \<times> data) option" where
-"step e s ip dt \<equiv>
-  case possible_steps e s ip dt of
+definition step :: "efsm \<Rightarrow> statename \<Rightarrow> label \<Rightarrow> inputs \<Rightarrow> data \<Rightarrow> (statename \<times> outvalues \<times> data) option" where
+"step e s l ip dt \<equiv>
+  case possible_steps e s l ip dt of
     [] \<Rightarrow> None
-    | [(s',(_,ops,ups))] \<Rightarrow> Some (s', ops (ip,dt), ups (ip,dt))
+    | [(s',t)] \<Rightarrow> Some (s', (outputs t) (ip,dt), (updates t) (ip,dt))
     | _ \<Rightarrow> None"
 declare step_def [simp]
 
 primrec observe_steps :: "efsm \<Rightarrow> statename \<Rightarrow> data \<Rightarrow> trace \<Rightarrow> observation" where
 "observe_steps _ _ _ [] = []"
 |"observe_steps e s dt (ip#ips) = 
-    (case step e s ip dt of
+    (case step e s (fst ip) (snd ip) dt of
       Some (s', ops, dt') \<Rightarrow> ops#(observe_steps e s' dt' ips)
       | None \<Rightarrow> []
     )"
 declare observe_steps_def [simp]
 
 definition observe :: "efsm \<Rightarrow> trace \<Rightarrow> observation" where
-"observe e tr \<equiv> observe_steps e (s0 e) (d0 e) tr"
+"observe e tr \<equiv> observe_steps e (s0 e) blankdata tr"
 
 definition equiv :: "efsm \<Rightarrow> efsm \<Rightarrow> trace \<Rightarrow> bool" where
 "equiv e1 e2 t \<equiv> (observe e1 t) = (observe e2 t)"
