formal/Vend.thy
@@ -3,24 +3,36 @@ theory Vend
 begin
 
 definition t1 :: "transition" where
-"t1 \<equiv> (\<lambda>(ip,dt) . ip(0) = Some (Inr ''select''), noouts, \<lambda>(ip,dt) . dt \<oplus> (1,ip(1)))"
+"t1 \<equiv> \<lparr> label = ''select'',
+        arity = 1,
+        guard = trueguard, 
+        outputs = noouts,
+        updates = \<lambda>(ip,dt) . dt \<oplus> (1,ip(1))
+      \<rparr>"
 
 abbreviation u1 :: "updates" where
 "u1 \<equiv> \<lambda>(ip,dt) . dt \<oplus> (2,(dt(2)) + (ip(1)))"
 
 definition t2 :: "transition" where
-"t2 \<equiv> (\<lambda>(ip,dt) . ip(0) = Some (Inr ''coin''), noouts, u1)"
-
-abbreviation g1 :: "guard" where
-"g1 \<equiv> \<lambda>(ip,dt) . (ip(0) = Some (Inr ''vend'')) \<and> (dt(2)) \<ge> (Some (Inl 100))"
+"t2 \<equiv> \<lparr> label = ''coin'',
+        arity = 1,
+        guard = trueguard, 
+        outputs = noouts,
+        updates = u1
+      \<rparr>"
 
 definition t3 :: "transition" where
-"t3 \<equiv> (g1, \<lambda>(ip,dt) . blankouts \<oplus> (1,dt(1)), noupdates)"
+"t3 \<equiv> \<lparr> label = ''vend'',
+        arity = 1,
+        guard = \<lambda>(ip,dt) . (dt(2)) \<ge> (Some (Inl 100)), 
+        outputs = \<lambda>(ip,dt) . blankouts \<oplus> (1,dt(1)),
+        updates = noupdates
+      \<rparr>"
 
 definition vend :: "efsm" where
 "vend \<equiv> \<lparr> S = [1,2,3],
           s0 = 1,
-          d0 = ((blankdata \<oplus> (1,Some (Inl 0))) \<oplus> (2,Some (Inl 0))),
+         (* d0 = ((blankdata \<oplus> (1,Some (Inl 0))) \<oplus> (2,Some (Inl 0))),*)
           M = \<lambda> (a,b) . 
               if (a,b) = (1,2) then [t1]
               else if (a,b) = (2,2) then [t2]
@@ -28,36 +40,36 @@ definition vend :: "efsm" where
               else []
          \<rparr>"
 
-lemma "possible_steps vend 1 blankips blankdata == []"
+lemma "possible_steps vend 1 ''coin'' blankips blankdata == []"
   by (simp add: vend_def t1_def)
-lemma "possible_steps vend 1 (blankips \<oplus> (0,Some (Inr ''select''))) blankdata == [(2,t1)]"
+lemma "possible_steps vend 1 ''select'' blankips blankdata == [(2,t1)]"
   by (simp add: vend_def t1_def)
-lemma "possible_steps vend 2 (blankips \<oplus> (0,Some (Inr ''coin''))) blankdata == [(2,t2)]"
+lemma "possible_steps vend 2 ''coin'' blankips blankdata == [(2,t2)]"
   by (simp add: vend_def t2_def t3_def)
-lemma "possible_steps vend 2 (blankips \<oplus> (0,Some (Inr ''vend''))) blankdata \<noteq> [(3,t3)]"
+lemma "possible_steps vend 2 ''vend'' blankips blankdata \<noteq> [(3,t3)]"
   by (simp add: vend_def t2_def t3_def)
-lemma "possible_steps vend 2 (blankips \<oplus> (0,Some (Inr ''vend''))) (blankdata \<oplus> (1,Some (Inl 50))) \<noteq> [(3,t3)]"
+lemma "possible_steps vend 2 ''vend'' blankips (blankdata \<oplus> (1,Some (Inl 50))) \<noteq> [(3,t3)]"
   by (simp add: vend_def t2_def t3_def)
-lemma "possible_steps vend 2 (blankips \<oplus> (0,Some (Inr ''vend''))) (blankdata \<oplus> (1,Some (Inl 99))) \<noteq> [(3,t3)]"
+lemma "possible_steps vend 2 ''vend'' blankips (blankdata \<oplus> (1,Some (Inl 99))) \<noteq> [(3,t3)]"
   by (simp add: vend_def t2_def t3_def)
-lemma "possible_steps vend 2 (blankips \<oplus> (0,Some (Inr ''vend''))) ((blankdata \<oplus> (1,Some (Inl 42))) \<oplus> (2,Some (Inl 100))) = [(3,t3)]"
+lemma "possible_steps vend 2''vend'' blankips ((blankdata \<oplus> (1,Some (Inl 42))) \<oplus> (2,Some (Inl 100))) = [(3,t3)]"
   by (simp add: vend_def t2_def t3_def)
 
-lemma "step vend 2 ((blankips \<oplus> (0,Some (Inr ''coin''))) \<oplus> (1,Some (Inl 50))) (blankdata \<oplus> (2,Some (Inl 0))) = Some (2, blankouts, (blankdata \<oplus> (2,Some (Inl 50))))"
+lemma "step vend 2 ''coin'' (blankips  \<oplus> (1,Some (Inl 50))) (blankdata \<oplus> (2,Some (Inl 0))) = Some (2, blankouts, (blankdata \<oplus> (2,Some (Inl 50))))"
   by (simp add: vend_def step_def t2_def t3_def) auto
 
 definition tr1 :: "trace" where
-"tr1 \<equiv> make_trace [[(Inr ''select''),(Inr ''coke'')],[(Inr ''coin''),(Inl 50)],[(Inr ''coin''),(Inl 50)],[(Inr ''vend'')]]"
+"tr1 \<equiv> make_trace [(''select'',[(Inr ''coke'')]),(''coin'',[(Inl 50)]),(''coin'',[(Inl 50)]),(''vend'',[])]"
 definition ob1 :: "observation" where
 "ob1 \<equiv> make_obs [[],[],[],[(Inr ''coke'')]]"
 
 definition tr2 :: "trace" where
-"tr2 \<equiv> make_trace [[(Inr ''select''),(Inr ''coke'')],[(Inr ''coin''),(Inl 50)],[(Inr ''coin''),(Inl 50)]]"
+"tr2 \<equiv> make_trace [(''select'',[(Inr ''coke'')]),(''coin'',[(Inl 50)]),(''coin'',[(Inl 50)])]"
 definition ob2 :: "observation" where
 "ob2 \<equiv> make_obs [[],[],[]]"
 
 definition tr3 :: "trace" where
-"tr3 \<equiv> make_trace [[(Inr ''select''),(Inl 42)]]"
+"tr3 \<equiv> make_trace [(''select'',[(Inl 42)])]"
 definition ob3 :: "observation" where
 "ob3 \<equiv> make_obs [[]]"
 
@@ -66,7 +78,7 @@ lemma "observe vend tr3 = ob3"
 
 lemma "observe vend tr2 = ob2" 
   by (simp add: vend_def tr2_def observe_def ob2_def t1_def t2_def t3_def)  
-  
+
 lemma "observe vend tr1 = ob1"
   by (simp add: vend_def tr1_def observe_def ob1_def t1_def t2_def t3_def)  
 
