formal/Vend2.thy
@@ -5,7 +5,6 @@ begin
 definition vend2 :: "efsm" where
 "vend2 \<equiv> \<lparr>S = [1,2,3,4],
           s0 = 1,
-          d0 = ((blankdata \<oplus> (1,Some (Inl 0))) \<oplus> (2,Some (Inl 0))),
           M = \<lambda>(s,s') . 
                 if (s,s') = (1,2) then [t1]
                 else if (s,s') = (2,3) then [t2]
@@ -14,7 +13,23 @@ definition vend2 :: "efsm" where
                 else []
           \<rparr>"
 
-theorem "equiv vend2 vend tr1"
+lemma "equiv vend2 vend tr1"
   by (simp add: t1_def t2_def t3_def vend_def vend2_def equiv_def observe_def tr1_def)
+
+theorem "equiv vend2 vend t"
+  apply (simp only: equiv_def observe_def)
+  apply (induct_tac "t")
+  using observe_steps.simps(1) apply auto[1]
+
+  apply (simp only: observe_steps_def)
+ 
+
+  apply (simp only: step_def)
+  apply (simp only: possible_steps_def)
+
+  apply (simp split: option.splits)
   
+  
+
+
 end
